Fix abstract pairwise proof

SimAsm/SimAsm.thy
@@ -1,182 +1,6 @@
 theory SimAsm
-  imports "../Soundness" 
+  imports  "../Soundness"  SimAsm_Exp
 begin
-
-section \<open>State\<close>
-
-datatype ('g,'r) var = Reg 'r | Glb 'g
-record ('v,'a) state_rec = st :: "'a \<Rightarrow> 'v"
-
-type_synonym ('v,'g,'r,'a) state = "('v,('g,'r) var,'a) state_rec_scheme"
-type_synonym ('v,'g,'a) gstate = "('v,'g,'a) state_rec_scheme"
-
-type_synonym ('v,'g,'r,'a) pred = "('v,'g,'r,'a) state set"
-type_synonym ('v,'g,'a) gpred = "('v,'g,'a) gstate set"
-
-type_synonym ('v,'g,'r,'a) trel = "('v,'g,'r,'a) state rel"
-type_synonym ('v,'g,'a) grel = "('v,'g,'a) gstate rel"
-
-type_synonym ('v,'g,'r,'a) trans = "('v,'g,'r,'a) pred \<Rightarrow> ('v,'g,'r,'a) pred"
-type_synonym ('v,'g,'r,'a) rtrans = "('v,'g,'r,'a) trel \<Rightarrow> ('v,'g,'r,'a) trel"
-
-type_synonym ('v,'g,'r,'a) auxfn = "('v,('g,'r) var,'a) state_rec_scheme \<Rightarrow> 'a"
-
-definition glb
-  where "glb m \<equiv> \<lambda>v. m (Glb v)"
-
-definition rg
-  where "rg m \<equiv> \<lambda>v. m (Reg v)"
-
-section \<open>Write Operations\<close>
-
-definition st_upd :: "('v,'a,'b) state_rec_scheme \<Rightarrow> 'a \<Rightarrow> 'v \<Rightarrow> ('v,'a,'b) state_rec_scheme"
-  where "st_upd m a b = m \<lparr> st := ((st m) (a := b)) \<rparr>"
-
-definition aux_upd :: "('v,'r,'a) state_rec_scheme \<Rightarrow> (('v,'r,'a) state_rec_scheme \<Rightarrow> 'a) \<Rightarrow> ('v,'r,'a) state_rec_scheme"
-  where "aux_upd m f \<equiv> m\<lparr>state_rec.more := f m\<rparr>"
-
-nonterminal updbinds and updbind
-
-syntax
-  "_updbindm" :: "'a \<Rightarrow> 'a \<Rightarrow> updbind"            ("(2_ :=\<^sub>s/ _)")
-  "_updbinda" :: "'a \<Rightarrow> updbind"                  ("(2aux:/ _)")
-  ""         :: "updbind \<Rightarrow> updbinds"             ("_")
-  "_updbinds":: "updbind \<Rightarrow> updbinds \<Rightarrow> updbinds" ("_,/ _")
-  "_Update"  :: "'a \<Rightarrow> updbinds \<Rightarrow> 'a"            ("_/'((_)')" [1000, 0] 900)
-
-translations
-  "_Update f (_updbinds b bs)" \<rightleftharpoons> "_Update (_Update f b) bs"
-  "f(x:=\<^sub>sy)" \<rightleftharpoons> "CONST st_upd f x y"
-  "f(aux: y)" \<rightleftharpoons> "CONST aux_upd f y"
-
-lemma [simp]:
-  "st (m(r :=\<^sub>s e)) q = (if r = q then e else st m q)"
-  by (auto simp: st_upd_def)
-
-lemma aux_nop [simp]:
-  "m(aux:more) = m"
-  by (auto simp: aux_upd_def)
-
-lemma st_upd_twist: "a \<noteq> c \<Longrightarrow> (m(a :=\<^sub>s b))(c :=\<^sub>s d) = (m(c :=\<^sub>s d))(a :=\<^sub>s b)"
-  unfolding st_upd_def by (auto intro!: equality fun_upd_twist)
-
-section \<open>Expression Language\<close>
-
-datatype ('v,'g,'r) exp = Var "('g,'r) var" | Val 'v | Exp "'v list \<Rightarrow> 'v" "('v,'g,'r) exp list"
-
-text \<open>Evaluate an expression given a state\<close>
-fun ev :: "('v,'g,'r,'a) state \<Rightarrow> ('v,'g,'r) exp \<Rightarrow> 'v"
-  where 
-    "ev m (Var r) = st m r" |
-    "ev _ (Val v) = v" |
-    "ev m (Exp f rs) = f (map (ev m) rs)"
-
-text \<open>The syntactic dependencies of an expression\<close>
-fun deps :: "('v,'g,'r) exp \<Rightarrow> ('g,'r) var set"
-  where 
-    "deps (Var r) = {r}" |
-    "deps (Exp _ rs) = \<Union>(deps ` set rs)" |
-    "deps _ = {}"
-
-text \<open>Substitute a variable for an expression\<close>
-fun subst :: "('v,'g,'r) exp \<Rightarrow> ('g,'r) var \<Rightarrow> ('v,'g,'r) exp \<Rightarrow> ('v,'g,'r) exp"
-  where
-    "subst (Var r) r' e = (if r = r' then e else Var r)" |
-    "subst (Exp f rs) r e = (Exp f (map (\<lambda>x. subst x r e) rs))" |
-    "subst e _ _ = e"
-
-datatype ('v,'g,'r) bexp = Neg "('v,'g,'r) bexp" | Exp\<^sub>B "'v list \<Rightarrow> bool" "('v,'g,'r) exp list"
-
-text \<open>Evaluate an expression given a state\<close>
-fun ev\<^sub>B :: "('v,'g,'r,'a) state \<Rightarrow> ('v,'g,'r) bexp \<Rightarrow> bool"
-  where 
-    "ev\<^sub>B m (Neg e) = (\<not> (ev\<^sub>B m e))" |
-    "ev\<^sub>B m (Exp\<^sub>B f rs) = f (map (ev m) rs)"
-
-text \<open>The syntactic dependencies of an expression\<close>
-fun deps\<^sub>B :: "('v,'g,'r) bexp \<Rightarrow> ('g,'r) var set"
-  where 
-    "deps\<^sub>B (Neg e) = deps\<^sub>B e" |
-    "deps\<^sub>B (Exp\<^sub>B _ rs) = \<Union>(deps ` set rs)"
-
-text \<open>Substitute a variable for an expression\<close>
-fun subst\<^sub>B :: "('v,'g,'r) bexp \<Rightarrow> ('g,'r) var \<Rightarrow> ('v,'g,'r) exp \<Rightarrow> ('v,'g,'r) bexp"
-  where
-    "subst\<^sub>B (Neg b) r e = Neg (subst\<^sub>B b r e)" |
-    "subst\<^sub>B (Exp\<^sub>B f rs) r e = (Exp\<^sub>B f (map (\<lambda>x. subst x r e) rs))"
-
-lemma [simp]:
-  "ev m (subst e r f) = ev (m(r :=\<^sub>s (ev m f))) e"
-proof (induct e)
-  case (Exp fn rs)
-  hence [simp]: "map (ev m \<circ> (\<lambda>x. subst x r f)) rs = map (ev (m(r :=\<^sub>s ev m f))) rs"
-    by auto
-  show ?case by simp
-qed auto
-
-lemma ev_nop [simp]:
-  "r \<notin> deps e \<Longrightarrow> ev (m(r :=\<^sub>s f)) e = ev m e"
-proof (induct e)
-  case (Exp fn rs)
-  hence [simp]: "map (ev (m(r :=\<^sub>s f))) rs = map (ev m) rs" by auto
-  show ?case by simp
-qed auto
-
-lemma [simp]:
-  "ev\<^sub>B m (subst\<^sub>B b r e) = ev\<^sub>B (m(r :=\<^sub>s (ev m e))) b"
-proof (induct b)
-  case (Exp\<^sub>B fn rs)
-  have [simp]: "map (ev m \<circ> (\<lambda>x. subst x r e)) rs = map (ev (m(r :=\<^sub>s ev m e))) rs"
-    by (auto simp: fun_upd_def)     
-  show ?case by simp
-qed simp
-
-lemma ev\<^sub>B_nop [simp]:
-  "r \<notin> deps\<^sub>B b \<Longrightarrow> ev\<^sub>B (m(r :=\<^sub>s f)) b = ev\<^sub>B m b"
-proof (induct b)
-  case (Exp\<^sub>B fn rs)
-  hence [simp]: "map (ev (m(r :=\<^sub>s f))) rs = map (ev m) rs"
-    using ev_nop[of r _ m f] by (auto simp: fun_upd_def) 
-  show ?case by simp
-qed simp
-
-section \<open>Operations\<close>
-
-datatype ('v,'g,'r) op =
-    assign "('g,'r) var" "('v,'g,'r) exp"
-  | cmp "('v,'g,'r) bexp"
-  | full_fence
-  | nop
-
-abbreviation ncmp
-  where "ncmp b \<equiv> cmp (Neg b)"
-
-fun beh\<^sub>i :: "('v,'g,'r) op \<Rightarrow> ('v,'g,'r,'a) state rel"
-  where
-    "beh\<^sub>i (assign a e) = {(m,m'). m' = m (a :=\<^sub>s ev m e)}" |
-    "beh\<^sub>i (cmp b) = {(m,m'). m = m' \<and> ev\<^sub>B m b}" |
-    "beh\<^sub>i _ = Id"
-
-text \<open>Variables written by an operation\<close>
-fun wr :: "('v,'g,'r) op \<Rightarrow> ('g,'r) var set"
-  where 
-    "wr (assign y _) = {y}" |
-    "wr _ = {}"
-
-text \<open>Variables read by an operation\<close>
-fun rd :: "('v,'g,'r) op \<Rightarrow> ('g,'r) var set"
-  where
-    "rd (assign _ e) = deps e" |
-    "rd (cmp b) = deps\<^sub>B b" |
-    "rd _ = {}"
-
-text \<open>Domain of register variables\<close>
-abbreviation locals
-  where "locals \<equiv> Reg ` UNIV"
-
-text \<open>Domain of register variables\<close>
-abbreviation globals
-  where "globals \<equiv> Glb ` UNIV"
 
 text \<open>Instruction Reordering\<close>
 text \<open>Only pattern match on first argument due to performance issues\<close>
@@ -186,19 +10,8 @@ fun re\<^sub>i :: "('v,'g,'r) op \<Rightarrow> ('v,'g,'r) op \<Rightarrow> bool"
     "re\<^sub>i (cmp b) \<alpha> = (\<alpha> \<noteq> full_fence \<and> wr \<alpha> \<subseteq> locals \<and> rd (cmp b) \<inter> wr \<alpha> = {} \<and> rd (cmp b) \<inter> rd \<alpha> \<subseteq> locals)" |
     "re\<^sub>i \<alpha> \<beta> = (\<beta> \<noteq> full_fence \<and> wr \<alpha> \<inter> wr \<beta> = {} \<and> rd \<alpha> \<inter> wr \<beta> = {} \<and> rd \<alpha> \<inter> rd \<beta> \<subseteq> locals)"
 
-text \<open>Sub-Instruction Forwarding\<close>
-fun fwd\<^sub>i :: "('v,'g,'r) op \<Rightarrow> ('v,'g,'r) op \<Rightarrow> ('v,'g,'r) op" 
-  where
-    "fwd\<^sub>i (assign r e) (assign r' e') = (assign r (subst e r' e'))" |
-    "fwd\<^sub>i (cmp b) (assign r e) = (cmp (subst\<^sub>B b r e))" |
-    "fwd\<^sub>i \<alpha> _ = \<alpha>"
-
-definition comp (infixr "\<Otimes>" 60)
-  where "comp a b \<equiv> {(m,m'). \<exists>m''. (m,m'') \<in> a \<and> (m'',m') \<in> b}"
-
-lemma re_consistent:
-  "re\<^sub>i \<alpha> (fwd\<^sub>i \<beta> \<alpha>) \<Longrightarrow> beh\<^sub>i \<alpha> \<Otimes> beh\<^sub>i \<beta> \<supseteq> beh\<^sub>i (fwd\<^sub>i \<beta> \<alpha>) \<Otimes> beh\<^sub>i \<alpha>"
-  by (cases \<alpha>; cases \<beta>, auto simp: comp_def intro!: st_upd_twist)
+fun fwd\<^sub>i  :: "('v,'g,'r) op \<Rightarrow> ('v,'g,'r) op \<Rightarrow> ('v,'g,'r) op" 
+  where "fwd\<^sub>i \<alpha> (assign x e) = subst\<^sub>i \<alpha> x e" | "fwd\<^sub>i \<alpha> _ = \<alpha>"
 
 section \<open>Auxiliary State Updates\<close>
 
@@ -211,22 +24,11 @@ This auxiliary state cannot influence real execution behaviour by definition.
 \<close>
 type_synonym ('v,'g,'r,'a) auxop = "('v,'g,'r) op \<times> ('v,'g,'r,'a) auxfn"
 
-(*
-lemma
-  "beh\<^sub>i (assign x (subst e y e')) = 
-    {(m,m'). \<exists>n. (m(y :=\<^sub>s ev m e'),n) \<in> beh\<^sub>i (assign x e) \<and> 
-                 m' = n(y :=\<^sub>s if x = y then st n y else st m y)}"
-  by (auto simp: st_upd_def intro!: equality)
-*)
-
 fun beh\<^sub>a :: "('v,'g,'r,'a) auxop \<Rightarrow> ('v,'g,'r,'a) state rel"
   where "beh\<^sub>a (\<alpha>,f) = beh\<^sub>i \<alpha> O {(m,m'). m' = m(aux: f)}"
 
 fun re\<^sub>a :: "('v,'g,'r,'a) auxop \<Rightarrow> ('v,'g,'r,'a) auxop \<Rightarrow> bool" 
-  where "re\<^sub>a (\<alpha>,f) (\<beta>,f') = re\<^sub>i \<alpha> \<beta>"
-
-fun fwd\<^sub>a :: "('v,'g,'r,'a) auxop \<Rightarrow> ('v,'g,'r,'a) auxop \<Rightarrow> ('v,'g,'r,'a) auxop" 
-  where "fwd\<^sub>a (\<alpha>,f) (\<beta>,f') = (fwd\<^sub>i \<alpha> \<beta>,f)"
+  where "re\<^sub>a (\<alpha>,_) (\<beta>,_) = re\<^sub>i \<alpha> \<beta>"
 
 section \<open>Instruction Specification Language\<close>
 
@@ -235,10 +37,11 @@ To instantiate the abstract theory, we must couple each sub-operation with its p
 and behaviour in a tuple\<close>
 type_synonym ('v,'g,'r,'a) opbasic = "(('v,'g,'r,'a) auxop, ('v,'g,'r,'a) state) basic"
 
-
 text \<open>Duplicate forwarding and reordering behaviour of underlying instruction\<close>
 fun fwd\<^sub>s :: "('v,'g,'r,'a) opbasic \<Rightarrow> ('v,'g,'r,'a) auxop \<Rightarrow> ('v,'g,'r,'a) opbasic" 
-  where "fwd\<^sub>s (\<alpha>,v,_) \<beta> =  (fwd\<^sub>a \<alpha> \<beta>, v, beh\<^sub>a (fwd\<^sub>a \<alpha> \<beta>))" 
+  where 
+    "fwd\<^sub>s ((\<alpha>,f),v,b) (assign x e,_) = (let p = (subst\<^sub>i \<alpha> x e, f) in  (p,v, beh\<^sub>a p))" |
+    "fwd\<^sub>s ((\<alpha>,f),v,b) (\<beta>,_) = ((\<alpha>,f),v,beh\<^sub>a (\<alpha>,f))"
 
 text \<open>Lift an operation with specification\<close>
 definition liftg :: "('v,'g,'r,'a) pred \<Rightarrow> ('v,'g,'r) op \<Rightarrow> ('v,'g,'r,'a) auxfn \<Rightarrow> ('v,'g,'r,'a) opbasic" 
