SimAsm/SimAsm_Exp.thy
@@ -1,0 +1,637 @@
+theory SimAsm_Exp
+  imports SimAsm_State
+begin
+
+section \<open>Expression Language\<close>
+
+datatype ('v,'g,'r) exp = Var "('g,'r) var" | Val 'v | Exp "'v list \<Rightarrow> 'v" "('v,'g,'r) exp list"
+
+text \<open>Evaluate an expression given a state\<close>
+fun ev\<^sub>E :: "('v,'g,'r,'a) state \<Rightarrow> ('v,'g,'r) exp \<Rightarrow> 'v"
+  where 
+    "ev\<^sub>E m (Var r) = st m r" |
+    "ev\<^sub>E _ (Val v) = v" |
+    "ev\<^sub>E m (Exp f rs) = f (map (ev\<^sub>E m) rs)"
+
+text \<open>The syntactic dependencies of an expression\<close>
+fun deps\<^sub>E :: "('v,'g,'r) exp \<Rightarrow> ('g,'r) var set"
+  where 
+    "deps\<^sub>E (Var r) = {r}" |
+    "deps\<^sub>E (Exp _ rs) = \<Union>(deps\<^sub>E ` set rs)" |
+    "deps\<^sub>E _ = {}"
+
+text \<open>Substitute a variable for an expression\<close>
+fun subst\<^sub>E :: "('v,'g,'r) exp \<Rightarrow> ('g,'r) var \<Rightarrow> ('v,'g,'r) exp \<Rightarrow> ('v,'g,'r) exp"
+  where
+    "subst\<^sub>E (Var r) r' e = (if r = r' then e else Var r)" |
+    "subst\<^sub>E (Exp f rs) r e = (Exp f (map (\<lambda>x. subst\<^sub>E x r e) rs))" |
+    "subst\<^sub>E e _ _ = e"
+
+datatype ('v,'g,'r) bexp = Neg "('v,'g,'r) bexp" | Exp\<^sub>B "'v list \<Rightarrow> bool" "('v,'g,'r) exp list"
+
+text \<open>Evaluate an expression given a state\<close>
+fun ev\<^sub>B :: "('v,'g,'r,'a) state \<Rightarrow> ('v,'g,'r) bexp \<Rightarrow> bool"
+  where 
+    "ev\<^sub>B m (Neg e) = (\<not> (ev\<^sub>B m e))" |
+    "ev\<^sub>B m (Exp\<^sub>B f rs) = f (map (ev\<^sub>E m) rs)"
+
+text \<open>The syntactic dependencies of an expression\<close>
+fun deps\<^sub>B :: "('v,'g,'r) bexp \<Rightarrow> ('g,'r) var set"
+  where 
+    "deps\<^sub>B (Neg e) = deps\<^sub>B e" |
+    "deps\<^sub>B (Exp\<^sub>B _ rs) = \<Union>(deps\<^sub>E ` set rs)"
+
+text \<open>Substitute a variable for an expression\<close>
+fun subst\<^sub>B :: "('v,'g,'r) bexp \<Rightarrow> ('g,'r) var \<Rightarrow> ('v,'g,'r) exp \<Rightarrow> ('v,'g,'r) bexp"
+  where
+    "subst\<^sub>B (Neg b) r e = Neg (subst\<^sub>B b r e)" |
+    "subst\<^sub>B (Exp\<^sub>B f rs) r e = (Exp\<^sub>B f (map (\<lambda>x. subst\<^sub>E x r e) rs))"
+
+section \<open>Operations\<close>
+
+datatype ('v,'g,'r) op =
+    assign "('g,'r) var" "('v,'g,'r) exp"
+  | cmp "('v,'g,'r) bexp"
+  | full_fence
+  | nop
+
+text \<open>Operation Behaviour\<close>
+fun beh\<^sub>i :: "('v,'g,'r) op \<Rightarrow> ('v,'g,'r,'a) state rel"
+  where
+    "beh\<^sub>i (assign a e) = {(m,m'). m' = m (a :=\<^sub>s ev\<^sub>E m e)}" |
+    "beh\<^sub>i (cmp b) = {(m,m'). m = m' \<and> ev\<^sub>B m b}" |
+    "beh\<^sub>i _ = Id"
+
+text \<open>Variables written by an operation\<close>
+fun wr :: "('v,'g,'r) op \<Rightarrow> ('g,'r) var set"
+  where 
+    "wr (assign y _) = {y}" |
+    "wr _ = {}"
+
+text \<open>Variables read by an operation\<close>
+fun rd :: "('v,'g,'r) op \<Rightarrow> ('g,'r) var set"
+  where
+    "rd (assign _ e) = deps\<^sub>E e" |
+    "rd (cmp b) = deps\<^sub>B b" |
+    "rd _ = {}"
+
+text \<open>Test if an instruction is a memory barrier\<close>
+fun barriers :: "('v,'g,'r) op \<Rightarrow> bool"
+  where "barriers full_fence = True" | "barriers _ = False"
+
+text \<open>Operation Substitution\<close>
+fun subst\<^sub>i :: "('v,'g,'r) op \<Rightarrow> ('g,'r) var \<Rightarrow> ('v,'g,'r) exp \<Rightarrow> ('v,'g,'r) op"
+  where
+    "subst\<^sub>i (assign x e) y f = assign x (subst\<^sub>E e y f)" |
+    "subst\<^sub>i (cmp b) y f = cmp (subst\<^sub>B b y f)" |
+    "subst\<^sub>i \<alpha> _ _ = \<alpha>"
+
+definition smap1
+  where "smap1 V x \<alpha> \<equiv> if x \<in> dom V then subst\<^sub>i \<alpha> x (Val (the (V x))) else \<alpha>"
+
+definition smap 
+  where "smap \<alpha> V \<equiv> Finite_Set.fold (smap1 V) \<alpha> (rd \<alpha>)"
+
+definition forall
+  where "forall V \<alpha> \<equiv> {smap \<alpha> M | M. dom M = V}"
+
+section \<open>Rules\<close>
+
+subsection \<open>Expression\<close>
+
+lemma ev_subst\<^sub>E [simp]:
+  "ev\<^sub>E m (subst\<^sub>E e r f) = ev\<^sub>E (m(r :=\<^sub>s (ev\<^sub>E m f))) e"
+proof (induct e)
+  case (Exp fn rs)
+  hence [simp]: "map (ev\<^sub>E m \<circ> (\<lambda>x. subst\<^sub>E x r f)) rs = map (ev\<^sub>E (m(r :=\<^sub>s ev\<^sub>E m f))) rs" by auto
+  show ?case by simp
+qed auto
+
+lemma subst_nop\<^sub>E [simp]:
+  "r \<notin> deps\<^sub>E e \<Longrightarrow> subst\<^sub>E e r f = e"
+proof (induct e)
+  case (Exp fn rs)
+  hence [simp]: "map (\<lambda>x. subst\<^sub>E x r f) rs = rs" by (induct rs) auto
+  show ?case by simp
+qed auto
+
+lemma ev_nop\<^sub>E [simp]:
+  "r \<notin> deps\<^sub>E e \<Longrightarrow> ev\<^sub>E (m(r :=\<^sub>s f)) e = ev\<^sub>E m e"
+proof (induct e)
+  case (Exp fn rs)
+  hence [simp]: "map (ev\<^sub>E (m(r :=\<^sub>s f))) rs = map (ev\<^sub>E m) rs" by auto
+  show ?case by simp
+qed auto
+
+lemma deps_subst\<^sub>E [simp]:
+  "deps\<^sub>E (subst\<^sub>E e x e') = deps\<^sub>E e - {x} \<union> (if x \<in> deps\<^sub>E e then deps\<^sub>E e' else {})"
+  by (induct e; auto simp: if_splits)
+
+lemma deps_ev\<^sub>E [intro]:
+  "\<forall>x \<in> deps\<^sub>E e. st m x = st m' x \<Longrightarrow> ev\<^sub>E m e = ev\<^sub>E m' e"
+proof (induct e)
+  case (Exp fn rs)
+  hence [simp]: "map (ev\<^sub>E m) rs = map (ev\<^sub>E m') rs" by (induct rs) auto
+  show ?case by simp
+qed auto
+
+lemma local_ev\<^sub>E [intro]:
+  "deps\<^sub>E e \<subseteq> locals \<Longrightarrow> rg m = rg m' \<Longrightarrow> ev\<^sub>E m e = ev\<^sub>E m' e"
+  apply (intro deps_ev\<^sub>E ballI, case_tac x)
+  by (auto simp: rg_def) metis
+
+lemma ev_aux\<^sub>E [simp]:
+  "ev\<^sub>E (x(aux: f)) g = ev\<^sub>E x g"
+proof (induct g)
+  case (Var x)
+  then show ?case by (auto simp: aux_upd_def)
+next
+  case (Val x)
+  then show ?case by (auto simp: aux_upd_def)
+next
+  case (Exp x1a x2a)
+  then show ?case by (metis (mono_tags, lifting) ev\<^sub>E.simps(3) map_eq_conv)
+qed
+
+lemma subst\<^sub>E_flip [simp]:
+  "x \<noteq> y \<Longrightarrow> subst\<^sub>E (subst\<^sub>E e x (Val v')) y (Val v) = subst\<^sub>E (subst\<^sub>E e y (Val v)) x (Val v')"
+  by (induct e) auto
+
+lemma subst\<^sub>E_rep [simp]:
+  "subst\<^sub>E (subst\<^sub>E e x (Val v')) x (Val v) = subst\<^sub>E e x (Val v')"
+  by (induct e) auto
+
+lemma finite_deps\<^sub>E [intro]:
+  "finite (deps\<^sub>E e)"
+  by (induct e) auto
+
+subsection \<open>Boolean Expression\<close>
+
+lemma ev_subst\<^sub>B [simp]:
+  "ev\<^sub>B m (subst\<^sub>B b r e) = ev\<^sub>B (m(r :=\<^sub>s (ev\<^sub>E m e))) b"
+proof (induct b)
+  case (Exp\<^sub>B fn rs)
+  have [simp]: "map (ev\<^sub>E m \<circ> (\<lambda>x. subst\<^sub>E x r e)) rs = map (ev\<^sub>E (m(r :=\<^sub>s ev\<^sub>E m e))) rs"
+    by (auto simp: fun_upd_def)     
+  show ?case by simp
+qed simp
+
+lemma ev_nop\<^sub>B [simp]:
+  "r \<notin> deps\<^sub>B b \<Longrightarrow> ev\<^sub>B (m(r :=\<^sub>s f)) b = ev\<^sub>B m b"
+proof (induct b)
+  case (Exp\<^sub>B fn rs)
+  hence [simp]: "map (ev\<^sub>E (m(r :=\<^sub>s f))) rs = map (ev\<^sub>E m) rs"
+    using ev_nop\<^sub>E[of r _ m f] by (auto simp: fun_upd_def) 
+  show ?case by simp
+qed simp
+
+lemma subst_nop\<^sub>B [simp]:
+  "r \<notin> deps\<^sub>B e \<Longrightarrow> subst\<^sub>B e r f = e"
+proof (induct e)
+  case (Exp\<^sub>B fn rs)
+  hence [simp]: "map (\<lambda>x. subst\<^sub>E x r f) rs = rs"  by (induct rs) auto
+  show ?case by simp
+qed auto
+
+lemma deps_subst\<^sub>B [simp]:
+  "deps\<^sub>B (subst\<^sub>B e x e') = deps\<^sub>B e - {x} \<union> (if x \<in> deps\<^sub>B e then deps\<^sub>E e' else {})"
+  by (induct e; auto simp: if_splits)
+
+lemma deps_ev\<^sub>B [intro]:
+  "\<forall>x \<in> deps\<^sub>B e. st m x = st m' x \<Longrightarrow> ev\<^sub>B m e = ev\<^sub>B m' e"
+proof (induct e)
+  case (Exp\<^sub>B fn rs)
+  hence [simp]: "map (ev\<^sub>E m) rs = map (ev\<^sub>E m') rs" by (induct rs) auto
+  show ?case by simp
+qed auto
+
+lemma ev_aux\<^sub>B [simp]:
+  "ev\<^sub>B (x(aux: f)) g = ev\<^sub>B x g"
+proof (induct g)
+  case (Neg g)
+  then show ?case by simp
+next
+  case (Exp\<^sub>B x1a x2)
+  then show ?case by (metis (no_types, lifting) ev\<^sub>B.simps(2) ev_aux\<^sub>E map_eq_conv)
+qed
+
+lemma subst\<^sub>B_flip [simp]:
+  "x \<noteq> y \<Longrightarrow> subst\<^sub>B (subst\<^sub>B e x (Val v')) y (Val v) = subst\<^sub>B (subst\<^sub>B e y (Val v)) x (Val v')"
+  by (induct e) auto
+
+lemma subst\<^sub>B_rep [simp]:
+  "subst\<^sub>B (subst\<^sub>B e x (Val v')) x (Val v) = subst\<^sub>B e x (Val v')"
+  by (induct e) auto
+
+lemma finite_deps\<^sub>B [intro]:
+  "finite (deps\<^sub>B e)"
+  by (induct e) auto
+
+subsection \<open>Operations\<close>
+
+lemma subst_wr [simp]:
+  "wr (subst\<^sub>i \<alpha> x e) = wr \<alpha>"
+  by (cases \<alpha>; auto)
+
+lemma subst_rd [simp]:
+  "rd (subst\<^sub>i \<alpha> x e) = rd \<alpha> - {x} \<union> (if x \<in> rd \<alpha> then deps\<^sub>E e else {})"
+  by (cases \<alpha>; auto)
+
+lemma subst_barriers [simp]:
+  "barriers (subst\<^sub>i \<alpha> x e) = barriers \<alpha>"
+  by (cases \<alpha>; auto)
+
+lemma subst_not_fence [simp]:
+  "(subst\<^sub>i \<alpha> x e \<noteq> full_fence) = (\<alpha> \<noteq> full_fence)"
+  by (cases \<alpha>; auto)
+
+lemma subst_nop [simp]:
+  "x \<notin> rd \<beta> \<Longrightarrow> subst\<^sub>i \<beta> x e = \<beta>"
+  unfolding smap1_def by (cases \<beta>) (auto split: if_splits)
+
+lemma finite_rd [intro]:
+  "finite (rd \<alpha>)"
+  by (cases \<alpha>) auto
+
+abbreviation ncmp
+  where "ncmp b \<equiv> cmp (Neg b)"
+
+subsection \<open>smap1 Theories\<close>
+
+lemma smap1_flip [simp]:
+  "smap1 V y (smap1 V x \<alpha>) = smap1 V x (smap1 V y \<alpha>)"
+  by (cases \<alpha>; cases "x = y"; auto simp: smap1_def)
+
+lemma smap1_rep [simp]:
+  "smap1 V x (smap1 V x \<alpha>) = smap1 V x \<alpha>"
+  by (cases \<alpha>; auto simp: smap1_def)
+
+interpretation cfi: comp_fun_idem "smap1 V"  by standard auto
+
+lemma smap1_rd [simp]:
+  "rd (smap1 M x \<beta>) = rd \<beta> - ({x} \<inter> dom M)"
+  unfolding smap1_def by (auto split: if_splits)
+
+lemma smap1_wr [simp]:
+  "wr (smap1 M x \<beta>) = wr \<beta>"
+  unfolding smap1_def by (auto split: if_splits)
+
+lemma smap1_barriers [simp]:
+  "barriers (smap1 M x \<beta>) = barriers \<beta>"
+  unfolding smap1_def by (auto split: if_splits)
+
+lemma smap1_nop [simp]:
+  "x \<notin> rd \<beta> \<Longrightarrow> smap1 M x \<beta> = \<beta>"
+  unfolding smap1_def by (auto split: if_splits)
+
+lemma smap1_nop2 [simp]:
+  "M x = None \<Longrightarrow> smap1 M x \<beta> = \<beta>"
+  unfolding smap1_def by (auto split: if_splits)
+
+lemma smap1_empty [simp]:
+  "smap1 Map.empty x \<beta> = \<beta>"
+  unfolding smap1_def by (auto split: if_splits)
+
+lemma smap1_fold_rd [simp]:
+  assumes "finite F"
+  shows "rd (Finite_Set.fold (smap1 M) \<beta> F) = rd \<beta> - (dom M \<inter> F)"
+  using assms
+proof (induct)
+  case empty
+  then show ?case by auto
+next
+  case (insert x F)
+  hence "Finite_Set.fold (smap1 M) \<beta> (insert x F) = smap1 M x (Finite_Set.fold (smap1 M) \<beta> F)"
+    using cfi.fold_insert_idem by blast
+  then show ?case by (auto simp: insert(3))
+qed
+
+lemma smap1_fold_wr [simp]:
+  assumes "finite F"
+  shows "wr (Finite_Set.fold (smap1 M) \<beta> F) = wr \<beta>"
+  using assms
+proof (induct)
+  case empty
+  then show ?case by auto
+next
+  case (insert x F)
+  hence "Finite_Set.fold (smap1 M) \<beta> (insert x F) = smap1 M x (Finite_Set.fold (smap1 M) \<beta> F)"
+    using cfi.fold_insert_idem by blast
+  then show ?case by (auto simp: insert(3))
+qed
+
+lemma smap1_fold_barriers [simp]:
+  assumes "finite F"
+  shows "barriers (Finite_Set.fold (smap1 M) \<beta> F) = barriers \<beta>"
+  using assms
+proof (induct)
+  case empty
+  then show ?case by auto
+next
+  case (insert x F)
+  hence "Finite_Set.fold (smap1 M) \<beta> (insert x F) = smap1 M x (Finite_Set.fold (smap1 M) \<beta> F)"
+    using cfi.fold_insert_idem by blast
+  then show ?case by (auto simp: insert(3))
+qed
+
+lemma smap1_fold_empty:
+  assumes "finite F"
+  shows "Finite_Set.fold (smap1 Map.empty) \<alpha> F = \<alpha>"
+  using assms
+proof (induct)
+  case empty
+  then show ?case by auto
+next
+  case (insert x F)
+  hence "Finite_Set.fold (smap1 Map.empty) \<alpha> (insert x F) = 
+         smap1 Map.empty x (Finite_Set.fold (smap1 Map.empty) \<alpha> F)"
+    using cfi.fold_insert_idem by blast
+  also have "... = Finite_Set.fold (smap1 Map.empty) \<alpha> F" by auto
+  also have "... = \<alpha>" using insert(3) by blast
+  finally show ?case .
+qed
+
+subsection \<open>smap Theories\<close>
+
+lemma smap_rd [simp]:
+  "rd (smap \<beta> M) = rd \<beta> - dom M"
+proof -
+  have "finite (rd \<beta>)" by auto
+  thus ?thesis unfolding smap_def by auto
+qed
+
+lemma smap_wr [simp]:
+  "wr (smap \<beta> M) = wr \<beta>"
+proof -
+  have "finite (rd \<beta>)" by auto
+  thus ?thesis unfolding smap_def by auto
+qed
+
+lemma smap_barriers [simp]:
+  "barriers (smap \<beta> M) = barriers \<beta>"
+proof -
+  have "finite (rd \<beta>)" by auto
+  thus ?thesis unfolding smap_def by auto
+qed
+
+lemma smap_empty [simp]:
+  "smap \<beta> Map.empty = \<beta>"
+proof -
+  have "finite (rd \<beta>)" by auto
+  thus ?thesis using smap1_fold_empty unfolding smap_def by auto
+qed
+
+lemma smap_rep [simp]:
+  "smap1 M x (smap \<beta> M) = smap \<beta> M"
+proof (cases "x \<in> rd \<beta>")
+  case True
+  have "Finite_Set.fold (smap1 M) \<beta> (insert x (rd \<beta>)) =
+        smap1 M x (Finite_Set.fold (smap1 M) \<beta> (rd \<beta>))"
+    using cfi.fold_insert_idem by blast
+  moreover have "insert x (rd \<beta>) = rd \<beta>" using True by auto
+  ultimately show ?thesis unfolding smap_def by auto
+next
+  case False
+  thus ?thesis by simp
+qed
+
+subsection \<open>forall Theories\<close>
+
+lemma forall_rd [simp]:
+  "\<forall>\<alpha> \<in> forall V \<beta>. rd \<alpha> = rd \<beta> - V"
+  unfolding forall_def by auto
+
+lemma forall_wr [simp]:
+  "\<forall>\<alpha> \<in> forall V \<beta>. wr \<alpha> = wr \<beta>"
+  unfolding forall_def by auto
+
+lemma forall_barriers [simp]:
+  "\<forall>\<alpha> \<in> forall V \<beta>. barriers \<alpha> = barriers \<beta>"
+  unfolding forall_def by auto
+
+lemma forall_fence [simp]:
+  "\<forall>\<alpha> \<in> forall V \<beta>.  (\<alpha> \<noteq> full_fence) = (\<beta> \<noteq> full_fence)"
+proof -
+  have "\<forall>\<alpha>. barriers \<alpha> = (\<alpha> = full_fence)" by (intro allI, case_tac \<alpha>; auto)
+  thus ?thesis using forall_barriers by blast
+qed
+
+lemma forall_nil [simp]:
+  "forall {} \<alpha> = {\<alpha>}"
+  unfolding forall_def by auto
+
+lemma smap1_cong [intro]:
+  "M x = N x \<Longrightarrow> smap1 M x = smap1 N x"
+  unfolding smap1_def using domIff by fastforce
+  
+lemma forall_unfold:
+  shows "forall (insert x V) \<alpha> = {subst\<^sub>i \<alpha>' x (Val c) | c \<alpha>'. \<alpha>' \<in> forall V \<alpha>}" (is "?L = ?R")
+proof -
+  have "?L \<subseteq> ?R"
+  proof (clarsimp simp: forall_def, cases "x \<in> V")
+    fix M assume d: "dom (M :: ('b, 'c) SimAsm_State.var \<Rightarrow> 'a option) = insert x V" "x \<in> V"
+    hence "smap \<alpha> M = subst\<^sub>i (smap \<alpha> M) x (Val (the (M x)))" by simp
+    moreover have "dom M = V" using d by auto
+    ultimately show "\<exists>c \<alpha>'. smap \<alpha> M = subst\<^sub>i \<alpha>' x (Val c) \<and> (\<exists>M. \<alpha>' = smap \<alpha> M \<and> dom M = V)"
+      by blast
+  next
+    fix M assume d: "dom (M :: ('b, 'c) SimAsm_State.var \<Rightarrow> 'a option) = insert x V" "x \<notin> V"
+    let ?M = "\<lambda>y. if x = y then None else M y"
+    have "smap \<alpha> M = subst\<^sub>i (smap \<alpha> ?M) x (Val (the (M x)))"
+    proof -
+      have mx: "Finite_Set.fold (smap1 M) \<alpha> (rd \<alpha> - {x}) = Finite_Set.fold (smap1 ?M) \<alpha> (rd \<alpha> - {x})"
+        by (auto intro!: Finite_Set.fold_cong simp add: cfi.comp_fun_commute_axioms)
+      show ?thesis
+      proof (cases "x \<in> rd \<alpha>")
+        case True
+        hence [simp]: "insert x (rd \<alpha>) = rd \<alpha>" by auto
+        have fx: "Finite_Set.fold (smap1 M) \<alpha> (insert x (rd \<alpha>)) = 
+                  smap1 M x (Finite_Set.fold (smap1 M) \<alpha> (rd \<alpha> - {x}))"
+          by (rule cfi.fold_insert_remove) blast
+        have "Finite_Set.fold (smap1 ?M) \<alpha> (insert x (rd \<alpha>)) = 
+                  smap1 ?M x (Finite_Set.fold (smap1 ?M) \<alpha> (rd \<alpha> - {x}))"
+          by (rule cfi.fold_insert_remove) blast
+        also have "... = Finite_Set.fold (smap1 ?M) \<alpha> (rd \<alpha> - {x})" by auto
+        finally show ?thesis using fx mx unfolding smap_def apply simp
+          unfolding smap1_def using d(1) by (auto split: if_splits)
+      next
+        case False
+        hence [simp]: "rd \<alpha> - {x} = rd \<alpha>" by auto
+        have "x \<notin> rd (smap \<alpha> ?M)" using False by simp
+        then show ?thesis using mx unfolding smap_def by simp
+      qed
+    qed
+    moreover have "dom ?M = V" using d by (auto split: if_splits)
+    ultimately show "\<exists>c \<alpha>'. smap \<alpha> M = subst\<^sub>i \<alpha>' x (Val c) \<and> (\<exists>M. \<alpha>' = smap \<alpha> M \<and> dom M = V)"
+      by blast
+  qed
+
+  moreover have "?R \<subseteq> ?L"
+  proof (clarsimp simp: forall_def, cases "x \<in> V")
+    fix M c assume d: "V = dom (M :: ('b, 'c) SimAsm_State.var \<Rightarrow> 'a option)" "x \<in> V" 
+    have "dom M = insert x (dom M)" using d by auto
+    moreover have "subst\<^sub>i (smap \<alpha> M) x (Val c) = smap \<alpha> M" using d by simp
+    ultimately show "\<exists>Ma. subst\<^sub>i (smap \<alpha> M) x (Val c) = smap \<alpha> Ma \<and> dom Ma = insert x (dom M)"
+      by blast
+  next
+    fix M c assume d: "V = dom (M :: ('b, 'c) SimAsm_State.var \<Rightarrow> 'a option)" "x \<notin> V" 
+    let ?M = "\<lambda>y. if y = x then Some c else M y"
+    have "dom ?M = insert x (dom M)" using d by auto
+    moreover have "subst\<^sub>i (smap \<alpha> M) x (Val c) = smap \<alpha> ?M"
+    proof -
+      have mx: "Finite_Set.fold (smap1 M) \<alpha> (rd \<alpha> - {x}) = Finite_Set.fold (smap1 ?M) \<alpha> (rd \<alpha> - {x})"
+        by (auto intro!: Finite_Set.fold_cong simp add: cfi.comp_fun_commute_axioms)
+      show ?thesis
+      proof (cases "x \<in> rd \<alpha>")
+        case True
+        hence [simp]: "insert x (rd \<alpha>) = rd \<alpha>" by auto
+        have fx: "Finite_Set.fold (smap1 ?M) \<alpha> (insert x (rd \<alpha>)) = 
+                  smap1 ?M x (Finite_Set.fold (smap1 ?M) \<alpha> (rd \<alpha> - {x}))"
+          by (rule cfi.fold_insert_remove) blast
+        have "Finite_Set.fold (smap1 M) \<alpha> (insert x (rd \<alpha>)) = 
+                  smap1 M x (Finite_Set.fold (smap1 M) \<alpha> (rd \<alpha> - {x}))"
+          by (rule cfi.fold_insert_remove) blast
+        also have "... = Finite_Set.fold (smap1 M) \<alpha> (rd \<alpha> - {x})" using d by auto        
+        finally show ?thesis using fx mx unfolding smap_def apply simp
+          unfolding smap1_def using d(1) by (auto split: if_splits)
+      next
+        case False
+        hence [simp]: "rd \<alpha> - {x} = rd \<alpha>" by auto
+        have "x \<notin> rd (smap \<alpha> ?M)" using False by simp
+        then show ?thesis using mx unfolding smap_def by simp
+      qed
+    qed
+    ultimately show "\<exists>Ma. subst\<^sub>i (smap \<alpha> M) x (Val c) = smap \<alpha> Ma \<and> dom Ma = insert x (dom M)"
+      by blast
+  qed
+
+  ultimately show ?thesis by blast
+qed
+
+lemma forall_one [simp]:
+  "forall {x} \<alpha> = {subst\<^sub>i \<alpha> x (Val c) | c. True}"
+  unfolding forall_unfold[of x "{}" \<alpha>] by auto
+
+lemma forall_nop [simp]:
+  assumes "x \<notin> rd \<alpha>" 
+  shows "forall (insert x V) \<alpha> = forall V \<alpha>"
+  using assms forall_unfold by force
+
+lemma forallI [intro]:
+  "smap \<alpha> M \<in> forall (dom M) \<alpha>"
+  by (auto simp: forall_def)
+
+subsection \<open>TODO\<close>
+
+definition upd
+  where "upd S f m \<equiv> m\<lparr>st := \<lambda>x. if x \<in> S then f x else st m x\<rparr>"
+
+lemma upd_nil [simp]:
+  "upd {} f m = m"
+  by (auto simp: upd_def)
+
+lemma upd_insert [simp]:
+  "upd (insert x V) f m = (upd V f m)(x :=\<^sub>s f x)"
+  by (auto simp: upd_def st_upd_def intro!: state_rec.equality)
+
+lemma upd_rep [simp]:
+  "upd A (st (upd A f m\<^sub>1)) m\<^sub>2 = upd A f m\<^sub>2"
+  by (auto simp: upd_def intro!: state_rec.equality)
+
+lemma upd_rep' [simp]:
+  "upd A f (upd B f m) = upd (A \<union> B) f m"
+  by (auto simp: upd_def intro!: state_rec.equality)
+
+lemma upd_st [simp]:
+  "st (upd S f m) x = (if x \<in> S then f x else st m x)"
+  by (auto simp: upd_def)
+
+lemma upd_more [simp]:
+  "state_rec.more (upd V f m) = state_rec.more m"
+  by (auto simp: upd_def)
+
+lemma st_upd_eq [intro]:
+  "state_rec.more m = state_rec.more m' \<Longrightarrow> \<forall>x. x \<noteq> y \<longrightarrow> st m x = st m' x \<Longrightarrow> m(y :=\<^sub>s e) = m'(y :=\<^sub>s e)"
+  by (auto simp: upd_def st_upd_def intro!: state_rec.equality)
+
+lemma beh_substi [simp]:
+  "beh\<^sub>i (subst\<^sub>i \<alpha> x e) = {(m\<^sub>1,upd (wr \<alpha>) (st m) m\<^sub>1) |m m\<^sub>1. (m\<^sub>1(x :=\<^sub>s ev\<^sub>E m\<^sub>1 e),m) \<in> beh\<^sub>i \<alpha>}"
+  apply (cases \<alpha>)
+  defer 1
+  apply (clarsimp simp: upd_def)
+  apply blast
+  apply (clarsimp simp: upd_def)
+  apply blast
+  apply (clarsimp simp: upd_def)
+  apply blast
+  apply (clarsimp simp: upd_def st_upd_def)
+  apply auto
+  apply (rule state_rec.equality)
+  apply auto
+  apply (rule state_rec.equality)
+  apply auto
+  done
+
+lemma [simp]:
+  "st (m(x :=\<^sub>s e)) = (st m)(x := e)"
+  by (auto simp: st_upd_def)
+
+lemma beh_smap1 [simp]:
+  "beh\<^sub>i (smap1 M x \<alpha>) = {(m\<^sub>1,upd (wr \<alpha>) (st m) m\<^sub>1) |m m\<^sub>1. (upd ({x} \<inter> dom M) (the o M) m\<^sub>1,m) \<in> beh\<^sub>i \<alpha>}"
+  by (cases \<alpha> ; auto simp: smap1_def)
+
+lemma beh_fold_smap1:
+  assumes "finite F" 
+  shows "beh\<^sub>i (Finite_Set.fold (smap1 M) \<alpha> F) = {(m\<^sub>1, upd (wr \<alpha>) (st m) m\<^sub>1) |m m\<^sub>1. (upd (F \<inter> dom M) (the \<circ> M) m\<^sub>1, m) \<in> beh\<^sub>i \<alpha>}"
+  using assms
+proof (induct)
+  case empty
+  then show ?case by (cases \<alpha> ; auto)
+next
+  case (insert x F)
+  hence f: "Finite_Set.fold (smap1 M) \<alpha> (insert x F) = 
+         smap1 M x (Finite_Set.fold (smap1 M) \<alpha> F)"
+    using cfi.fold_insert_idem by blast
+
+  show ?case using insert(1)
+    unfolding f beh_smap1 insert(3)
+    apply auto unfolding o_def 
+    apply (intro exI conjI)
+    apply blast
+    apply (metis Int_Un_distrib2 Un_insert_right inf_bot_right sup_inf_absorb)
+    apply (intro exI conjI)
+    prefer 2
+    apply blast
+    apply simp
+    apply (metis Int_Un_distrib2 Un_insert_right inf_bot_right sup_inf_absorb)
+    done
+qed
+
+lemma beh_smap [simp]:
+  "beh\<^sub>i (smap \<alpha> M) = {(m\<^sub>1,upd (wr \<alpha>) (st m) m\<^sub>1) | m m\<^sub>1. (upd (dom M) (the o M) m\<^sub>1,m) \<in> beh\<^sub>i \<alpha>}"
+proof -
+  have "finite (rd \<alpha>)" by auto
+  hence "beh\<^sub>i (Finite_Set.fold (smap1 M) \<alpha> (rd \<alpha>)) = 
+          {(m\<^sub>1, upd (wr \<alpha>) (st m) m\<^sub>1) |m m\<^sub>1. (upd ((rd \<alpha>) \<inter> dom M) (the \<circ> M) m\<^sub>1, m) \<in> beh\<^sub>i \<alpha>}"
+    using beh_fold_smap1 by blast
+
+  also have "... = {(m\<^sub>1, upd (wr \<alpha>) (st m) m\<^sub>1) |m m\<^sub>1. (upd (dom M) (the \<circ> M) m\<^sub>1, m) \<in> beh\<^sub>i \<alpha>}"
+    apply (cases \<alpha>; auto)
+    apply (rule equality; auto)
+    apply fastforce
+    apply (rule equality; auto)
+    apply fastforce
+    apply (subgoal_tac "ev\<^sub>B (upd (deps\<^sub>B x2 \<inter> dom M) (the \<circ> M) m\<^sub>1) x2 = ev\<^sub>B (upd (dom M) (the \<circ> M) m\<^sub>1) x2")
+    apply blast
+    apply (rule deps_ev\<^sub>B)
+    apply auto
+    apply (subgoal_tac "ev\<^sub>B (upd (deps\<^sub>B x2 \<inter> dom M) (the \<circ> M) m\<^sub>1) x2 = ev\<^sub>B (upd (dom M) (the \<circ> M) m\<^sub>1) x2")
+    apply blast
+    apply (rule deps_ev\<^sub>B)
+    apply auto
+    done
+
+  finally show ?thesis unfolding smap_def .
+qed
+
+end
